systems/Disk.v
@@ -10,7 +10,8 @@ Section Disk.
   Context {orig_failure_params : FailureParams orig_multi_params}.
   Context {data_serializer : Serializer data}.
 
-  Definition init_disk h := serialize_top (serialize (init_handlers h)).
+  Definition init_disk (h : name) : IOStreamWriter.wire :=
+    serialize_top (serialize (init_handlers h)).
   
   Definition disk_net_handlers dst src m st :=
     let '(out, data, ps) := net_handlers dst src m st in
@@ -20,12 +21,7 @@ Section Disk.
     let '(out, data, ps) := input_handlers h inp st in
     (serialize_top (serialize data), out, data, ps).
 
-  Instance disk_base_params : BaseParams :=
-    {
-      data := data ;
-      input := input ;
-      output := output
-    }.
+  Instance disk_base_params : BaseParams := orig_base_params.
 
   Instance disk_multi_params : DiskMultiParams disk_base_params :=
     {
@@ -46,11 +42,12 @@ Section Disk.
   Instance disk_failure_params : DiskFailureParams disk_multi_params :=
     {
       d_reboot :=
-        fun s =>
-          match deserialize_top deserialize s with
-          | Some d => Some (@reboot _ _ orig_failure_params d)
-          | None => None
-          end
+        fun n s =>
+          reboot
+            (match deserialize_top deserialize s with
+              | Some d => d
+              | None => init_handlers n
+             end)
     }.
 End Disk.
 
